\documentclass{article}
\author{Hugo Thomas \\ \texttt{hugo.thomas@tuta.io}}
\usepackage[utf8]{inputenc}
\usepackage{ bbm }
\usepackage{ geometry}
\geometry{legalpaper, margin=1.3in}

\title{Signals and Communications}

\begin{document}
\maketitle
\tableofcontents
\newpage
\section{Signals and systems}
\subsection*{Dirac Impluse Relation}
$$
    f(t)\delta(t-t_0)=f(t_0)\delta(t-t_0)
$$

\subsection*{Energy of a continuous-time signal}
$$
E = \int_{-\infty}^{+\infty}x(t)x^*(t)dt
$$

\subsection*{Mean power of a continuous-time signal}
$$
P_x = \lim_{\theta \to +\infty} \frac{1}{2\theta}
\int_{-\theta}^{+\theta}x(t)x^*(t)dt
$$

\begin{center}
This is equal to $0$ if $x(t)$ is an energy-type signal.
\end{center}


\subsection*{Correlations}
\begin{table}[h]
\begin{tabular}{lll}
& \multicolumn{1}{c}{Cross-correlation} & \multicolumn{1}{c}{Auto-correlation} \\
energy-type & $\gamma_{xy}(\tau) = \int_{-\infty}^{+\infty}x(t)y^*(t-\tau)dt$ & $\gamma_{xx}(\tau) = \int_{-\infty}^{+\infty}x(t)x^*(t-\tau)dt$ \\
power-type & $\gamma_{xy}(\tau) = \frac{1}{2\theta}\int_{-\theta}^{+\theta}x(t)y^*(t-\tau)dt$ & $\gamma_{xx}(\tau) = \frac{1}{2\theta}\int_{-\theta}^{+\theta}x(t)x^*(t-\tau)dt $
\end{tabular}
\end{table}

\subsection*{Linearity and time-invariance}
A system is linear iff:
$$
    \forall x_i(t), \forall a_i \in \mathbbm{R} \quad f(\sum_i a_ix_i) = \sum_ia_if(x_i)
$$

\subsection*{Convolution}
$$
y(t)=x(t)*h(t)=\int_{-\infty}^{_\infty}x(t-u)h(u)du
$$

\subsection*{Time shift}
$$
x(t)\delta(t-\tau)=x(t-\tau)
$$
\newpage
\section{The Fourier Transform}
\subsection*{Fourier transform of a continuous-time signal}
$$
X(f)=FT\{x(t)\}=\int_{-\infty}^{+\infty}x(t)e^{-j2\pi ft}dt
$$

\subsection*{Inverse Fourier transform of a continuous-time signal}
$$
x(t)=FT^{-1}\{X(f)\} = \int_{-\infty}^{_\infty}X(f)e^{+j2\pi ft}df
$$

\subsection*{Properties of the Fourier Transform}
\subsubsection*{time shifting}
$$
FT\{x(t-\tau)\}=e^{+j2\pi ft}X(f)
$$
\subsubsection*{time reversal}
$$
FT\{x(-t)\}=X(-f)
$$
\subsubsection*{conjugation}
$$
FT\{x^*(t)\}=X^*(-f)
$$

\subsection*{Fourier transform of a covolution product}
$$
FT\{x(t)*y(t)\}=X(f)Y(f)
$$
\end{document}
